remove Cond and related definitions

Blanc/ReSolvent.lean
@@ -20,9 +20,6 @@ def State.Solvent (w : State) (a : Adr) : Prop :=
 def Devm.getStor (devm : Devm) (adr : Adr) : Stor :=
   (devm.getAcct adr).stor
 
-def Devm.Solvent (devm : Devm) (a : Adr) (sevm : Sevm) : Prop :=
-  (sevm.currentTarget = a → Stor.Solvent (devm.getStor a) sevm.value (devm.getBal a)) ∧
-  (sevm.currentTarget ≠ a → Stor.Solvent (devm.getStor a) 0 (devm.getBal a))
 
 def Devm.PreSolvent (devm : Devm) (a : Adr) (sevm : Sevm) : Prop :=
   (sevm.currentTarget = a → Stor.Solvent (devm.getStor a) sevm.value (devm.getBal a)) ∧
@@ -30,15 +27,6 @@ def Devm.PreSolvent (devm : Devm) (a : Adr) (sevm : Sevm) : Prop :=
 
 def Devm.PostSolvent (devm : Devm) (a : Adr) : Prop :=
   Stor.Solvent (devm.getStor a) 0 (devm.getBal a)
-
-def Execution.Solvent (sevm : Sevm) : Execution → Adr → Prop
-  | .error _, _ => True
-  | .ok devm, adr => devm.Solvent adr sevm
-
--- Cond : invariant in the main induction for proof of solvency preservation
-structure Cond (wa : Adr) (sevm : Sevm) (devm : Devm) : Prop where
-  (nof : sum devm.getBal < 2 ^ 256)
-  (solvent : devm.Solvent wa sevm)
 
 structure Precond (wa : Adr) (sevm : Sevm) (devm : Devm) : Prop where
   (nof : sum devm.getBal < 2 ^ 256)
@@ -48,13 +36,13 @@ structure Postcond (wa : Adr) (sevm : Sevm) (devm : Devm) : Prop where
   (nof : sum devm.getBal < 2 ^ 256)
   (solvent : devm.PostSolvent wa)
 
-lemma Postcond.of_cond {wa : Adr} {sevm : Sevm} {devm : Devm}
-    (h : Cond wa sevm devm) : Postcond wa sevm devm := by
+lemma postcond_of_precond {wa : Adr} {sevm : Sevm} {devm : Devm}
+    (h : Precond wa sevm devm) : Postcond wa sevm devm := by
   constructor
   · exact h.nof
   · unfold Devm.PostSolvent
     have h_solv := h.solvent
-    unfold Devm.Solvent at h_solv
+    unfold Devm.PreSolvent at h_solv
     by_cases hc : sevm.currentTarget = wa
     · have h1 := h_solv.left hc
       unfold Stor.Solvent at h1
@@ -63,36 +51,9 @@ lemma Postcond.of_cond {wa : Adr} {sevm : Sevm} {devm : Devm}
       omega
     · exact h_solv.right hc
 
-lemma Cond.of_precond {wa : Adr} {sevm : Sevm} {devm : Devm}
-    (h : Precond wa sevm devm) : Cond wa sevm devm := by
-  constructor
-  · exact h.nof
-  · exact h.solvent
-
-lemma Postcond.of_precond {wa : Adr} {sevm : Sevm} {devm : Devm}
-    (h : Precond wa sevm devm) : Postcond wa sevm devm :=
-  Postcond.of_cond (Cond.of_precond h)
-
-lemma Precond.state_eq_pp {wa sevm devm devm'}
+lemma Precond.state_eq {wa sevm devm devm'}
     (h_pc : Precond wa sevm devm) (h_eq : devm'.state = devm.state) :
     Precond wa sevm devm' := by
-  cases h_pc with
-  | mk h_nof h_solv =>
-    have h_bal : devm'.getBal = devm.getBal := by
-      funext a; simp [Devm.getBal, Devm.getAcct]; rw [h_eq]
-    have h_stor : ∀ a, devm'.getStor a = devm.getStor a := by
-      intro a; simp [Devm.getStor, Devm.getAcct]; rw [h_eq]
-    constructor
-    · rw [h_bal]; exact h_nof
-    · cases h_solv with
-      | intro hl hr =>
-        constructor
-        · intro h; rw [h_bal, h_stor wa]; exact hl h
-        · intro h; rw [h_bal, h_stor wa]; exact hr h
-
-lemma Precond.state_eq {wa sevm devm devm'}
-    (h_pc : Cond wa sevm devm) (h_eq : devm'.state = devm.state) :
-    Cond wa sevm devm' := by
   cases h_pc with
   | mk h_nof h_solv =>
     have h_bal : devm'.getBal = devm.getBal := by
@@ -120,17 +81,14 @@ class Hinv1 {ξ υ} (r : Devm → ξ)
     (f : Devm → Except (String × Devm) (υ × Devm)) where
   (inv : Inv1 r f)
 
-def Exec.InvDepth (k : Nat) (ca : Adr) (p : Prog) (σ : Sevm → Devm → Prop) : Prop :=
-  ForallDeeperAt k ca p (λ _ sevm pre exn _ => σ sevm pre → ifOk (σ sevm) exn)
-
-def Exec.InvDepth_pp (k : Nat) (ca : Adr) (p : Prog)
+def Exec.InvDepth (k : Nat) (ca : Adr) (p : Prog)
   (σ : Sevm → Devm → Prop) (ρ : Sevm → Devm → Prop) : Prop :=
   ForallDeeperAt k ca p (λ _ sevm pre exn _ => σ sevm pre → ifOk (ρ sevm) exn)
 
 lemma Line.inv_solvent {e e' s l s' a}
     (h_bal : Line.Inv Devm.getBal l) (h_stor : Line.Inv Devm.getStor l)
-    (h_sv : Devm.Solvent s a e) (h_run : Line.Run e' s l s') : Devm.Solvent s' a e := by
-  unfold Devm.Solvent; rw [← h_bal h_run, ← h_stor h_run]; exact h_sv
+    (h_sv : Devm.PreSolvent s a e) (h_run : Line.Run e' s l s') : Devm.PreSolvent s' a e := by
+  unfold Devm.PreSolvent; rw [← h_bal h_run, ← h_stor h_run]; exact h_sv
 
 lemma chargeGas_getBal_eq {cost devm devm'} (h : chargeGas cost devm = .ok devm') : devm.getBal = devm'.getBal := by
   dsimp [chargeGas] at h
@@ -390,75 +348,16 @@ instance : Ninst.Hinv Devm.state (Ninst.reg Rinst.gt) := ⟨by
           exact hs1.trans (hs2.trans hs3)
 ⟩
 
-
 lemma deposit_inv_solvent {sevm : Sevm} {s r : Devm}
     (run : Func.Run (weth.main :: weth.aux) sevm s deposit r)
     (h_sv : s.PreSolvent sevm.currentTarget sevm) :
-    r.Solvent sevm.currentTarget sevm := sorry
+    r.PostSolvent sevm.currentTarget := sorry
 
 lemma Func.inv_nof {c : List Func} {sevm : Sevm} {s r : Devm} {f : Func}
     (run : Func.Run c sevm s f r) (h_nof : sum s.getBal < 2 ^ 256) :
     sum r.getBal < 2 ^ 256 := sorry
 
-lemma name_inv_solvent {sevm : Sevm} {s r : Devm}
-    (run : Func.Run (weth.main :: weth.aux) sevm s name r)
-    (h_sv : s.Solvent sevm.currentTarget sevm) :
-    r.Solvent sevm.currentTarget sevm := sorry
-
-lemma approve_inv_solvent {sevm : Sevm} {s r : Devm}
-    (run : Func.Run (weth.main :: weth.aux) sevm s approve r)
-    (h_sv : s.Solvent sevm.currentTarget sevm) :
-    r.Solvent sevm.currentTarget sevm := sorry
-
-lemma totalSupply_inv_solvent {sevm : Sevm} {s r : Devm}
-    (run : Func.Run (weth.main :: weth.aux) sevm s totalSupply r)
-    (h_sv : s.Solvent sevm.currentTarget sevm) :
-    r.Solvent sevm.currentTarget sevm := sorry
-
-lemma transferFrom_inv_solvent {sevm : Sevm} {s r : Devm}
-    (run : Func.Run (weth.main :: weth.aux) sevm s transferFrom r)
-    (h_sv : s.Solvent sevm.currentTarget sevm) :
-    r.Solvent sevm.currentTarget sevm := sorry
-
-lemma withdraw_inv_solvent {sevm : Sevm} {s r : Devm}
-    (cond : Cond sevm.currentTarget sevm s)
-    (ih : Exec.InvDepth sevm.depth sevm.currentTarget weth (Cond sevm.currentTarget))
-    (run : Func.Run (weth.main :: weth.aux) sevm s withdraw r) :
-    r.Solvent sevm.currentTarget sevm := sorry
-
-lemma withdraw_inv_solvent_pp {sevm : Sevm} {s r : Devm}
-    (cond : Precond sevm.currentTarget sevm s)
-    (ih : Exec.InvDepth_pp sevm.depth sevm.currentTarget weth (Precond sevm.currentTarget) (Postcond sevm.currentTarget))
-    (run : Func.Run (weth.main :: weth.aux) sevm s withdraw r) :
-    r.Solvent sevm.currentTarget sevm := sorry
-
-
-lemma decimals_inv_solvent {sevm : Sevm} {s r : Devm}
-    (run : Func.Run (weth.main :: weth.aux) sevm s decimals r)
-    (h_sv : s.Solvent sevm.currentTarget sevm) :
-    r.Solvent sevm.currentTarget sevm := sorry
-
-lemma balanceOf_inv_solvent {sevm : Sevm} {s r : Devm}
-    (run : Func.Run (weth.main :: weth.aux) sevm s balanceOf r)
-    (h_sv : s.Solvent sevm.currentTarget sevm) :
-    r.Solvent sevm.currentTarget sevm := sorry
-
-lemma symbol_inv_solvent {sevm : Sevm} {s r : Devm}
-    (run : Func.Run (weth.main :: weth.aux) sevm s symbol r)
-    (h_sv : s.Solvent sevm.currentTarget sevm) :
-    r.Solvent sevm.currentTarget sevm := sorry
-
-lemma transfer_inv_solvent {sevm : Sevm} {s r : Devm}
-    (run : Func.Run (weth.main :: weth.aux) sevm s transfer r)
-    (h_sv : s.Solvent sevm.currentTarget sevm) :
-    r.Solvent sevm.currentTarget sevm := sorry
-
-lemma allowance_inv_solvent {sevm : Sevm} {s r : Devm}
-    (run : Func.Run (weth.main :: weth.aux) sevm s allowance r)
-    (h_sv : s.Solvent sevm.currentTarget sevm) :
-    r.Solvent sevm.currentTarget sevm := sorry
-
-lemma run_inv_cond_pp (f : Func)
+lemma run_inv_cond (f : Func)
     ( h_solv :
       ∀ {sevm : Sevm} {s r : Devm},
         Func.Run (weth.main :: weth.aux) sevm s f r →
@@ -473,19 +372,10 @@ lemma run_inv_cond_pp (f : Func)
   · apply Func.inv_nof run cond.nof
   · apply h_solv run cond.solvent
 
-lemma run_inv_cond (f : Func)
-    (h_solv : ∀ {sevm : Sevm} {s r : Devm}, Func.Run (weth.main :: weth.aux) sevm s f r → s.Solvent sevm.currentTarget sevm → r.Solvent sevm.currentTarget sevm) :
-    ∀ {sevm : Sevm} {s r : Devm}, Func.Run (weth.main :: weth.aux) sevm s f r →
-      Cond sevm.currentTarget sevm s → Cond sevm.currentTarget sevm r := by
-  intro sevm s r run cond
-  constructor
-  · apply Func.inv_nof run cond.nof
-  · apply h_solv run cond.solvent
-
-lemma weth_inv'_pp {sevm : Sevm} {s r}
+lemma weth_inv {sevm : Sevm} {s r}
     (cond : Precond sevm.currentTarget sevm s)
     ( ih :
-      Exec.InvDepth_pp sevm.depth sevm.currentTarget weth
+      Exec.InvDepth sevm.depth sevm.currentTarget weth
         (Precond sevm.currentTarget)
         (Postcond sevm.currentTarget) ) :
     Func.Run (weth.main :: weth.aux) sevm s (Func.call 0) r →
@@ -498,7 +388,7 @@ lemma weth_inv'_pp {sevm : Sevm} {s r}
   rename Devm => s₀
   cases eq
   have cond₀ : Precond sevm.currentTarget sevm s₀ :=
-    Precond.state_eq_pp cond burn.state.symm
+    Precond.state_eq cond burn.state.symm
   clear cond burn s
   revert run
   pexec fsig
@@ -511,89 +401,18 @@ lemma weth_inv'_pp {sevm : Sevm} {s r}
   clear s₀
   intro temp
   apply
-    ( @dispatchWith_inv_pp
+    ( @dispatchWith_inv
       (weth.main :: weth.aux) 1 deposit
       (λ e s =>
          Precond e.currentTarget e s ∧
-         Exec.InvDepth_pp e.depth e.currentTarget weth (Precond e.currentTarget) (Postcond e.currentTarget) )
+         Exec.InvDepth e.depth e.currentTarget weth (Precond e.currentTarget) (Postcond e.currentTarget) )
       (λ e r => Postcond e.currentTarget e r)
-
       ?_ ?_ rfl ?_ wethTree ?_ sevm s₁ r ⟨cond₁, ih⟩ temp )
     <;> clear temp cond₁ ih r s₁ sevm
   · intro e s x w s' s'' ⟨h_cond, h_ih⟩ h_run h_pop
     refine' ⟨_, h_ih⟩
     have h_run_state : s.state = s'.state := Line.of_inv Devm.state (by line_inv) h_run
     rcases h_pop with ⟨_, _, _, _, _, _, _, _, _, _, _, h_pop_state, _⟩
-    apply Precond.state_eq_pp h_cond
-    exact h_pop_state.symm.trans h_run_state.symm
-  · intro e s x w s' s'' ⟨h_cond, h_ih⟩ h_run h_pop
-    refine' ⟨_, h_ih⟩
-    have h_run_state : s.state = s'.state := Line.of_inv Devm.state (by line_inv) h_run
-    rcases h_pop with ⟨_, _, _, _, _, _, _, _, _, _, _, h_pop_state, _⟩
-    apply Precond.state_eq_pp h_cond
-    exact h_pop_state.symm.trans h_run_state.symm
-  · intro e s s' r ⟨cond, ih⟩ burn run
-    have cond' : Precond e.currentTarget e s' := Precond.state_eq_pp cond burn.state.symm
-    have cond_c : Cond e.currentTarget e s' := Cond.of_precond cond'
-    have r_cond : Cond e.currentTarget e r := run_inv_cond deposit deposit_inv_solvent run cond_c
-    exact Postcond.of_cond r_cond
-  · intro e s r wf h_mem ⟨cond, ih⟩ h_run
-    rcases h_mem with (((h | h) | h) | (h | h)) | (((h | h) | h) | (h | h)) <;>
-      (cases h)
-    · apply Postcond.of_cond <| run_inv_cond name name_inv_solvent h_run (Cond.of_precond cond)
-    · apply Postcond.of_cond <| run_inv_cond approve approve_inv_solvent h_run (Cond.of_precond cond)
-    · apply Postcond.of_cond <| run_inv_cond totalSupply totalSupply_inv_solvent h_run (Cond.of_precond cond)
-    · apply Postcond.of_cond <| run_inv_cond transferFrom transferFrom_inv_solvent h_run (Cond.of_precond cond)
-    · have r_cond : Cond e.currentTarget e r := ⟨Func.inv_nof h_run cond.nof, withdraw_inv_solvent_pp cond ih h_run⟩
-      exact Postcond.of_cond r_cond
-    · apply Postcond.of_cond <| run_inv_cond decimals decimals_inv_solvent h_run (Cond.of_precond cond)
-    · apply Postcond.of_cond <| run_inv_cond balanceOf balanceOf_inv_solvent h_run (Cond.of_precond cond)
-    · apply Postcond.of_cond <| run_inv_cond symbol symbol_inv_solvent h_run (Cond.of_precond cond)
-    · apply Postcond.of_cond <| run_inv_cond transfer transfer_inv_solvent h_run (Cond.of_precond cond)
-    · apply Postcond.of_cond <| run_inv_cond allowance allowance_inv_solvent h_run (Cond.of_precond cond)
-
-
-lemma weth_inv' {sevm : Sevm} {s r}
-    (cond : Cond sevm.currentTarget sevm s)
-    (ih : Exec.InvDepth sevm.depth sevm.currentTarget weth (Cond sevm.currentTarget)) :
-    Func.Run (weth.main :: weth.aux) sevm s (Func.call 0) r →
-    Cond sevm.currentTarget sevm r := by
-
-  -- unwrap the initial `call 0` (this part does not exist in original proof in Solvent.lean)
-  intro run; cases run
-  rename (_ = _) => eq
-  rename (Func.Run _ _ _ _ _) => run
-  rename (Devm.Burn _ _) => burn
-  rename Devm => s₀
-  cases eq
-  have cond₀ : Cond sevm.currentTarget sevm s₀ :=
-    Precond.state_eq cond burn.state.symm
-  clear cond burn s
-  revert run
-
-  -- this point corresponds to the starting point of weth_inv' in Solvent.lean
-
-  pexec fsig
-  have cond₁  : Cond sevm.currentTarget sevm s₁ := by
-    refine' ⟨_, _⟩
-    · rw [← Line.of_inv Devm.getBal (by line_inv) h₁]; exact cond₀.nof
-    · apply Line.inv_solvent _ _ cond₀.solvent h₁ <;> line_inv
-  clear cond₀
-  clear h₁
-  clear s₀
-  intro temp
-  apply
-    ( @dispatchWith_inv
-      (weth.main :: weth.aux) 1 deposit
-      (λ e s =>
-         Cond e.currentTarget e s ∧
-         Exec.InvDepth e.depth e.currentTarget weth (Cond e.currentTarget) )
-      ?_ ?_ rfl ?_ wethTree ?_ sevm s₁ r ⟨cond₁, ih⟩ temp ).1
-    <;> clear temp cond₁ ih r s₁ sevm
-  · intro e s x w s' s'' ⟨h_cond, h_ih⟩ h_run h_pop
-    refine' ⟨_, h_ih⟩
-    have h_run_state : s.state = s'.state := Line.of_inv Devm.state (by line_inv) h_run
-    rcases h_pop with ⟨_, _, _, _, _, _, _, _, _, _, _, h_pop_state, _⟩
     apply Precond.state_eq h_cond
     exact h_pop_state.symm.trans h_run_state.symm
   · intro e s x w s' s'' ⟨h_cond, h_ih⟩ h_run h_pop
@@ -603,40 +422,36 @@ lemma weth_inv' {sevm : Sevm} {s r}
     apply Precond.state_eq h_cond
     exact h_pop_state.symm.trans h_run_state.symm
   · intro e s s' r ⟨cond, ih⟩ burn run
-    refine' ⟨_, ih⟩
-    have cond' : Cond e.currentTarget e s' := Precond.state_eq cond burn.state.symm
-    apply run_inv_cond deposit deposit_inv_solvent run cond'
+    have cond' : Precond e.currentTarget e s' := Precond.state_eq cond burn.state.symm
+    --have cond_c : Cond e.currentTarget e s' := Cond.of_precond cond'
+    have r_cond : Postcond e.currentTarget e r :=
+      run_inv_cond deposit deposit_inv_solvent run cond'
+    exact r_cond
   · intro e s r wf h_mem ⟨cond, ih⟩ h_run
-    refine' ⟨_, ih⟩
     rcases h_mem with (((h | h) | h) | (h | h)) | (((h | h) | h) | (h | h)) <;>
       (cases h)
-    · apply run_inv_cond name name_inv_solvent h_run cond
-    · apply run_inv_cond approve approve_inv_solvent h_run cond
-    · apply run_inv_cond totalSupply totalSupply_inv_solvent h_run cond
-    · apply run_inv_cond transferFrom transferFrom_inv_solvent h_run cond
-    · refine' ⟨Func.inv_nof h_run cond.nof, withdraw_inv_solvent cond ih h_run⟩
-    · apply run_inv_cond decimals decimals_inv_solvent h_run cond
-    · apply run_inv_cond balanceOf balanceOf_inv_solvent h_run cond
-    · apply run_inv_cond symbol symbol_inv_solvent h_run cond
-    · apply run_inv_cond transfer transfer_inv_solvent h_run cond
-    · apply run_inv_cond allowance allowance_inv_solvent h_run cond
-
-
-
-
-
+    · sorry
+    · sorry
+    · sorry
+    · sorry
+    · sorry
+    · sorry
+    · sorry
+    · sorry
+    · sorry
+    · sorry
 
 theorem weth_inv_solvent (wa : Adr) :
     ∀ sevm pre post,
       Exec 0 sevm pre (.ok post)  →
       (sevm.currentTarget = wa → some sevm.code.toList = Prog.compile weth) →
-      Cond wa sevm pre →
-      Cond wa sevm post := by
+      Precond wa sevm pre →
+      Postcond wa sevm post := by
   intro sevm devm exn exc h_code h_pc
-  apply lift_inv wa weth (Cond wa) --(Postcond wa)
+  apply lift_inv wa weth (Precond wa) (Postcond wa)
   · intro sevm pre post run eq; rw [← eq]
     dsimp [Prog.Run] at run
-    intro ih cond; apply weth_inv' cond _ run
+    intro ih cond; apply weth_inv cond _ run
     intro pc' sevm' devm' exn'
     cases exn'; {simp only [ifOk, implies_true]}
     apply ih
